src/crypto/aes/x64/Low.GCMencrypt.fst
@@ -133,7 +133,7 @@ let aes128_encrypt_block_buffer
      output_q == aes_encrypt_LE AES_128 (Ghost.reveal key) input_q)
   )         
   =
-  AESEncryptBlock.aes128_encrypt_block output_b input_b key keys_b
+  AESEncryptBlock_win.aes128_encrypt_block_win output_b input_b key keys_b
   
 let aes128_encrypt_block_BE_buffer 
              (input_b output_b:B.buffer U8.t) 
@@ -160,7 +160,7 @@ let aes128_encrypt_block_BE_buffer
      output_q == aes_encrypt_BE AES_128 (Ghost.reveal key) input_q)
   )   
   =
-  AESEncryptBE.aes128_encrypt_block_be output_b input_b key keys_b
+  AESEncryptBE_win.aes128_encrypt_block_be_win output_b input_b key keys_b
 
 let gctr_bytes_extra_buffer
              (plain_b:B.buffer U8.t) (num_bytes:U64.t) 
@@ -227,7 +227,7 @@ let gctr_bytes_extra_buffer
     )
   ) 
   = 
-  GCTR.gctr_bytes_extra_buffer plain_b num_bytes iv_old iv_b key keys_b cipher_b
+  GCTR_win.gctr_bytes_extra_buffer_win plain_b num_bytes iv_old iv_b key keys_b cipher_b
 
 let ghash_incremental_bytes_buffer (h_b hash_b input_b:B.buffer U8.t) (num_bytes:U64.t) : Stack unit
   (requires fun h -> 
@@ -259,7 +259,7 @@ let ghash_incremental_bytes_buffer (h_b hash_b input_b:B.buffer U8.t) (num_bytes
     )
   )
   =
-  GHash_stdcall.ghash_incremental_bytes_stdcall h_b hash_b input_b num_bytes
+  GHash_stdcall_win.ghash_incremental_bytes_stdcall_win h_b hash_b input_b num_bytes
 
 let ghash_incremental_one_block_buffer (h_b hash_b input_b:B.buffer U8.t) (offset:U64.t) : Stack unit
   (requires fun h -> 
@@ -286,7 +286,7 @@ let ghash_incremental_one_block_buffer (h_b hash_b input_b:B.buffer U8.t) (offse
     )
   )
   =
-  GHash_one_block.ghash_incremental_one_block_buffer h_b hash_b input_b offset
+  GHash_one_block_win.ghash_incremental_one_block_buffer_win h_b hash_b input_b offset
 
 let ghash_incremental_bytes_extra_buffer
              (in_b hash_b h_b:B.buffer U8.t) (num_bytes:U64.t) 
@@ -343,7 +343,7 @@ let ghash_incremental_bytes_extra_buffer
     )
   ) 
   =
-  GHash_extra.ghash_incremental_extra_stdcall in_b hash_b h_b num_bytes orig_hash
+  GHash_extra_win.ghash_incremental_extra_stdcall_win in_b hash_b h_b num_bytes orig_hash
 
 let gcm_load_xor_store_buffer
        (plain_b mask_b cipher_b:B.buffer U8.t) 
@@ -397,8 +397,7 @@ let gcm_load_xor_store_buffer
   =
   let num_blocks = Ghost.hide (U64.v (Ghost.reveal num_blocks)) in
   let h = ST.get() in
-// TODO: Weaken this  
-  Gcm_load_xor.gcm_load_xor_store_buffer plain_b mask_b cipher_b offset num_blocks key iv
+  Gcm_load_xor_win.gcm_load_xor_store_buffer_win plain_b mask_b cipher_b offset num_blocks key iv
 
 let inc32_buffer (iv_b:B.buffer U8.t) : Stack unit
   (requires fun h ->
@@ -411,7 +410,7 @@ let inc32_buffer (iv_b:B.buffer U8.t) : Stack unit
      let new_iv = buffer_to_quad32 iv_b h' in
      new_iv == inc32 old_iv 1))
   =
-  Inc32.inc32_buffer iv_b
+  Inc32_win.inc32_buffer_win iv_b
   
 let zero_quad32_buffer (b:B.buffer U8.t) : Stack unit
   (requires fun h ->
@@ -424,7 +423,7 @@ let zero_quad32_buffer (b:B.buffer U8.t) : Stack unit
      new_b == Mkfour 0 0 0 0)
   )
   = 
-  Zero_quad32.zero_quad32_buffer b
+  Zero_quad32_win.zero_quad32_buffer b
   
 let mk_quad32_lo0_be_1_buffer (b:B.buffer U8.t) : Stack unit
   (requires fun h ->
@@ -438,7 +437,7 @@ let mk_quad32_lo0_be_1_buffer (b:B.buffer U8.t) : Stack unit
      new_b == Mkfour 1 old_b.lo1 old_b.hi2 old_b.hi3)
   )
   =
-  Mk_quad32_1.mk_quad32_lo0_be_1_buffer b
+  Mk_quad32_1_win.mk_quad32_lo0_be_1_buffer_win b
 
 let gcm_make_length_quad_buffer 
   (plain_num_bytes auth_num_bytes:U64.t)
@@ -456,7 +455,7 @@ let gcm_make_length_quad_buffer
      new_b == reverse_bytes_quad32 (Mkfour (8 * (U64.v plain_num_bytes)) 0 (8 * (U64.v auth_num_bytes)) 0))
   )
   = 
-  Gcm_make_length.gcm_make_length_quad_buffer plain_num_bytes auth_num_bytes b
+  Gcm_make_length_win.gcm_make_length_quad_buffer_win plain_num_bytes auth_num_bytes b
 
 
 let quad32_xor_buffer 
@@ -480,7 +479,7 @@ let quad32_xor_buffer
      dst = quad32_xor src1 src2)
   )
   =
-  Quad32_xor.quad32_xor_buffer src1 src2 dst
+  Quad32_xor_win.quad32_xor_buffer_win src1 src2 dst
   
 (*** Actual Low* code ***)
 
